Quo lemmas

ztest.sml
@@ -13,9 +13,6 @@ AX1 |> qspecl [‘N * N’,‘N * N’] |> uex2ex_rule
     |> store_as "ZR_def";
 
 
-strip_quants
-
-val f = “!a:mem(N * N). P(a)”
 
 fun dest_cross t = 
     case view_term t of 
@@ -52,7 +49,42 @@ fun forall_cross_fconv f =
     in dimpI l2r r2l 
     end
 
-val f = “?a:mem(A * B).P(a)”
+
+
+val f = “∀b':mem(N * N).P(a:mem(N),b:mem(N),b')”;
+val f = “∀a1 a2 a3. Holds(ZR,a1,a2) & Holds(ZR,z2,z3)”;
+
+fun forall_cross_fconv f = 
+    let val (pv as (n,s),b) = dest_forall f 
+        val pset = s |> dest_sort |> #2  |> hd
+        val (A,B) = dest_cross pset 
+        val pt = mk_var pv
+        val eth = Pair_has_comp |> specl [A,B,pt]
+        val (ocv1 as (ocn1,ocs1),ob1) = dest_exists (concl eth) 
+        val (ocv2 as (ocn2,ocs2),ob2) = dest_exists ob1
+        val avoids = fvf b
+        val ct1 = pvariantt avoids (mk_var ocv1)
+        val ct2 = pvariantt avoids (mk_var ocv2)
+        val (cv1 as (cn1,cs1)) = dest_var ct1
+        val (cv2 as (cn2,cs2)) = dest_var ct2
+        val b1 = substf (ocv1,ct1) ob1
+        val b2 = substf (ocv2,ct2) (substf (ocv1,ct1) ob2)
+        val pair = mk_Pair ct1 ct2 
+        val b' = substf (pv,pair) b
+        val new = mk_forall cn1 cs1 (mk_forall cn2 cs2 b')
+        val l2r = f |> assume |> allE pair 
+                    |> simple_genl [cv1,cv2]
+                    |> disch f
+        val eth1 = b1 |> assume 
+        val r2l = new |> assume |> specl [ct1,ct2]
+                      |> rewr_rule[GSYM $ assume b2]
+                      |> existsE cv2 eth1 
+                      |> existsE cv1 eth
+                      |> allI pv
+                      |> disch new
+    in dimpI l2r r2l 
+    end
+
 
 fun exists_cross_fconv f = 
     let val (pv as (n,s),b) = dest_exists f 
@@ -82,31 +114,11 @@ fun exists_cross_fconv f =
                     |> disch new
     in dimpI l2r r2l
     end
-                    |> existsI cv2 ct2 b'
-                    |> existsI cv1 ct1 new0
-                    |> existsE cv2 (assume b1)
-                    |> existsE cv1 eth
-                    |> existsE pv (assume f)
-                    |> disch f
 
-val (a,s) = cv1;
-val t = ct1 ;
-val f = b1;
-val (G,A,C) = dest_thm 
-(b |> assume |> rewr_rule[assume b2]
-                    |> existsI cv2 ct2 b')
-f |> assume |> allE pair 
-                    |> simple_genl [cv1,cv2]
-                    |> disch f
-        val eth1 = b1 |> assume 
-        val r2l = new |> assume |> specl [ct1,ct2]
-                      |> rewr_rule[GSYM $ assume b2]
-                      |> existsE cv2 eth1 
-                      |> existsE cv1 eth
-                      |> allI pv
-                      |> disch new
-    in dimpI l2r r2l 
-    end
+
+(*depth_fconv no_conv forall_cross_fconv “!a:mem(N * N) b:mem(N * N). P(a,b)”
+not doing the desired thing *)
+
 
 val ZR_Refl = prove_store("ZR_Refl",
 e0
@@ -116,43 +128,84 @@ e0
  “Refl(ZR)”));
 
 
+fun basic_fconv_tac c fc = fconv_tac $ basic_fconv c fc
+fun depth_fconv_tac c fc = fconv_tac $ depth_fconv c fc
+
+(*use add_sub*)
+val ZR_Trans = prove_store("ZR_Trans",
+e0
+(rw[Trans_def] >> depth_fconv_tac no_conv forall_cross_fconv >>
+ rw[ZR_def] >> 
+ qsuff_tac
+ ‘!a1 b1 a2 b2 a3 b3.
+  Add(a1,b2) = Add(a2,b1) & Add(a2,b3) = Add(a3,b2) ==>
+  Add(a1,b3) = Add(a3,b1)’
+ >-- rw[] >>
+ rpt strip_tac >>
+ irule Add_eq_eq >> qexists_tac ‘b2’ >>
+ once_rw[GSYM Add_assoc] >>
+ qby_tac
+ ‘Add(b3,b2) = Add(b2,b3) & Add(b1,b2) = Add(b2,b1)’ 
+ >-- (strip_tac 
+     >-- qspecl_then [‘b2’,‘b3’] accept_tac Add_comm
+     >-- qspecl_then [‘b2’,‘b1’] accept_tac Add_comm) >>
+ arw[] >>
+ rw[Add_assoc] >> once_arw[] >> 
+ qpick_x_assum ‘Add(a2, b3) = Add(a3, b2)’
+ (assume_tac o GSYM) >> once_arw[] >>
+ rw[GSYM Add_assoc] >>
+ qspecl_then [‘b3’,‘b1’] assume_tac Add_comm >>
+ once_arw[] >> rw[])
+(form_goal
+ “Trans(ZR)”));
+
+ 
+val ZR_Sym = prove_store("ZR_Sym",
+e0
+(rw[Sym_def] >> depth_fconv_tac no_conv forall_cross_fconv >>
+ rw[ZR_def] >>  rpt strip_tac >> arw[])
+(form_goal
+ “Sym(ZR)”));
+
 
 val ZR_ER = prove_store("ZR_ER",
 e0
-(cheat)
+(rw[ER_def,ZR_Sym,ZR_Refl,ZR_Trans])
 (form_goal “ER(ZR)”));
 
 
-val Sg_ex = prove_store("Sg_ex",
-e0
-(cheat)
-(form_goal “!A. ?Sg:A-> Pow(A). 
- !a a'.IN(a',App(Sg,a)) <=> a' = a”));
 
-val Sg_def = Sg_ex |> spec_all |> qSKOLEM"Sg" [‘A’] 
-                   |> gen_all
+val Sg_def = P2fun'|> qspecl [‘A’,‘Pow(A)’] 
+                   |> fVar_sInst_th “P(a:mem(A),s:mem(Pow(A)))”
+                      “!a0. IN(a0,s) <=> a0 = a:mem(A)”
+                   |> C mp 
+                      (IN_def_P |> spec_all
+                                |> fVar_sInst_th “P(a0:mem(A))”
+                                   “a0 = a:mem(A)”
+                                |> qgen ‘a’)
+                   |> qSKOLEM "Sg" [‘A’] |> gen_all
                    |> store_as "Sg_def";
-
-
-val Sing_ex = prove_store("Sing_ex",
-e0
-(cheat)
-(form_goal
- “!A a:mem(A).?sa. sa = App(Sg(A),a)”));
 
 val Sing_def = qdefine_fsym ("Sing",[‘a:mem(A)’])
                             ‘App(Sg(A),a:mem(A))’
                             |> gen_all |> store_as "Sing_def";
 
 
-val Ri_ex = prove_store("Ri_ex",
-e0
-(cheat)
-(form_goal “!A B r:A~>B. ?Ri:Pow(A) -> Pow(B).
- !s b. IN(b,App(Ri,s)) <=> ?a. IN(a,s) & Holds(r,a,b)”));
+val Ri_def = P2fun'|> qspecl [‘Pow(A)’,‘Pow(B)’] 
+                   |> fVar_sInst_th “P(sa:mem(Pow(A)),sb:mem(Pow(B)))”
+                      “!b. IN(b,sb) <=> ∃a. IN(a,sa) & Holds(r:A~>B,a,b)”
+                   |> C mp 
+                      (IN_def_P |> qspecl [‘B’]
+                                |> fVar_sInst_th “P(b:mem(B))”
+                                   “∃a. IN(a,sa) & Holds(r:A~>B,a,b)”
+                                |> qgen ‘sa’)
+                   |> qSKOLEM "Ri" [‘r’] |> gen_all
+                   |> qspecl [‘A’,‘B’,‘r:A~>B’,‘s:mem(Pow(A))’]
+                   |> qgenl [‘A’,‘B’,‘r’,‘s’]
+                   |> store_as "Ri_def";
 
-val Ri_def = Ri_ex |> spec_all |> qSKOLEM "Ri" [‘r’] 
-                   |> gen_all |> store_as "Ri_def";
+
+
 
 (*Relational singleton image*)
 val Rsi_def = qdefine_fsym ("Rsi",[‘r:A~>B’])
@@ -164,13 +217,32 @@ val rsi_def = qdefine_fsym ("rsi",[‘r:A~>B’,‘a:mem(A)’])
                             ‘App(Rsi(r),a)’
                             |> gen_all |> store_as "rsi_def";
 
+val IN_rsi = prove_store("IN_rsi",
+e0
+(rw[rsi_def,Rsi_def,Ri_def,App_App_o,Sg_def] >>
+ rpt strip_tac >> dimp_tac >> strip_tac >> rfs[] >>
+ qexists_tac ‘a1’ >> arw[])
+(form_goal “∀A r:A~>A a1 a2. IN(a2,rsi(r,a1)) ⇔ Holds(r,a1,a2) ”));
 
 
+val ER_Holds = prove_store("ER_Holds",
+e0
+(rpt strip_tac >> dimp_tac >> rpt strip_tac (* 2 *)
+ >-- (first_x_assum (qspecl_then [‘a2’] assume_tac) >> fs[ER_def,Refl_def]) >>
+ dimp_tac >> strip_tac >> fs[ER_def,Sym_def,Trans_def] (* 2 *)
+ >-- (first_x_assum irule >> qexists_tac ‘a1’ >> arw[] >> first_x_assum irule >>
+     arw[]) >>
+ first_x_assum irule >> qexists_tac ‘a2’ >> arw[])
+(form_goal “∀A r:A~>A. ER(r) ⇒ ∀a1 a2. 
+ ((∀x.Holds(r,a1,x) ⇔ Holds(r,a2,x)) ⇔ Holds(r,a1,a2))”));
+ 
 val rsi_eq_ER = prove_store("rsi_eq_ER",
 e0
-(cheat)
+(rw[GSYM IN_EXT_iff,IN_rsi] >> 
+ rpt strip_tac >> drule ER_Holds >> arw[])
 (form_goal “!A r:A~>A.ER(r) ==> 
  !a1 a2. rsi(r,a1) = rsi(r,a2) <=> Holds(r,a1,a2)”));
+
 
 
 val Z_def = Thm_2_4 |> qspecl [‘Pow(N * N)’]
@@ -202,8 +274,7 @@ e0
  first_x_assum (drule o iffRL) >>
  pop_assum strip_assume_tac >>
  qsspecl_then [‘n’] strip_assume_tac Pair_has_comp >>
- fs[] >> qexistsl_tac [‘a’,‘b’] >> arw[]
- )
+ fs[] >> qexistsl_tac [‘a’,‘b’] >> arw[])
 (form_goal 
  “!z:mem(Z).?m n. App(iZ,z) = rsi(ZR,Pair(m,n))”));
 
@@ -224,33 +295,35 @@ val resp_def =
  |> gen_all |> store_as "resp_def";
 
 
+val rext_def = AX1 |> qspecl [‘Pow(A)’,‘Pow(B)’] 
+                   |> fVar_sInst_th “P(sa:mem(Pow(A)),sb:mem(Pow(B)))”
+                      “?a b.sa = rsi(r1:A~>A,a) & sb = rsi(r2:B~>B,b) & 
+                            App(f,a) = b”
+                   |> uex2ex_rule
+                   |> qSKOLEM "rext" [‘f’,‘r1’,‘r2’]
+                   |> gen_all |> store_as "rext_def";                       
 
 
-val rext_ex = prove_store("rext_ex",
-e0
-(cheat)
-(form_goal
- “!A B f:A->B r1:A~>A r2:B~>B.
- ?e:Pow(A) ~> Pow(B).
-  !sa sb. Holds(e,sa,sb) <=> 
-   ?a b.sa = rsi(r1,a) & sb = rsi(r2,b) &
-    App(f,a) = b”));
+val prrel_def = AX1 |> qspecl [‘A * B’,‘A * B’]
+                    |> fVar_sInst_th “P(ab1:mem(A * B),ab2:mem(A * B))”
+                       “Holds(r1:A~>A,Fst(ab1),Fst(ab2)) &
+                        Holds(r2:B~>B,Snd(ab1),Snd(ab2))”
+                    |> uex2ex_rule |> qSKOLEM "prrel" [‘r1’,‘r2’]
+                    |> qspecl [‘Pair(a1:mem(A),b1:mem(B))’,
+                               ‘Pair(a2:mem(A),b2:mem(B))’]
+                    |> rewr_rule[Pair_def']
+                    |> qgenl [‘A’,‘r1’,‘B’,‘r2’,‘a1’,‘b1’,‘a2’,‘b2’]
+                    |> store_as "prrel_def";
 
-val rext_def = rext_ex |> spec_all 
-                       |> qSKOLEM "rext"
-                       [‘f’,‘r1’,‘r2’]
-                       |> gen_all |> store_as "rext_def";
 
-(* product rel *)
-val prrel_ex = prove_store("prrel_ex",
-e0
-(cheat)
-(form_goal “!A r1:A~>A B r2:B~>B. ?r:A * B ~> A * B.
- !a1 b1 a2 b2.Holds(r,Pair(a1,b1),Pair(a2,b2)) <=> 
- Holds(r1,a1,a2) & Holds(r2,b1,b2)”));
+(*
+we really want to check only resp, not biresp, so 
+  App(Image(f#), rsi(r1#, a#)) = rsi(r2#, App(f#, a#)) 
+is wrong, it is only:
+  App(Image(f#), rsi(r1#, a#)) ⊆ rsi(r2#, App(f#, a#)):
+ Larry is not claiming it as well, Larry is using Abs_Integ o Image(f), which is only one direction of the implication
 
-val prrel_def = prrel_ex |> spec_all |> qSKOLEM "prrel"
-[‘r1’,‘r2’] |> gen_all |> store_as "prrel_def";
+*)
 
 
 
@@ -267,33 +340,43 @@ e0
  strip_tac >> 
  qby_tac
  ‘!sb.(?!q2. sb = App(i2,q2)) <=> 
-       ?b. sb = rsi(r2,b)’ >-- cheat (* easy by injection*)>>
+       ?b. sb = rsi(r2,b)’ >-- 
+ (strip_tac >> dimp_tac >> disch_tac 
+ >-- (pop_assum (assume_tac o uex2ex_rule) >> 
+     first_x_assum (drule o iffLR) >> arw[]) >>
+ uex_tac >> first_x_assum (drule o iffRL) >>
+ pop_assum strip_assume_tac >> qexists_tac ‘q2’ >> arw[] >>
+ rpt strip_tac >> fs[Inj_def] >> first_x_assum irule >> arw[])
+ (* easy by injection*)>>
  fs[resp_def] >>
  first_x_assum (qspecl_then [‘App(i1,x)’] assume_tac) >>
- qby_tac ‘?a. App(i1,x) = rsi(r1,a)’ >-- cheat >>
+ qby_tac ‘?a. App(i1,x) = rsi(r1,a)’ >-- 
+ (first_x_assum (irule o iffLR) >> qexists_tac ‘x’ >> rw[]) >>
  (*should be auto*)
- pop_assum strip_assume_tac >>
+ pop_assum strip_assume_tac >> 
  first_x_assum (qspecl_then [‘App(Rsi(r2) o f,a)’] 
  assume_tac) >> fs[GSYM rsi_def,App_App_o] >>
  qby_tac
  ‘?!q2:mem(Q2). rsi(r2, App(f, a)) = App(i2, q2)’
- >-- cheat >>
+ >-- (first_x_assum (irule o iffRL) >> qexists_tac ‘App(f,a)’ >> rw[]) >>
  qsuff_tac ‘!q2:mem(Q2). 
   rsi(r2, App(f, a)) = App(i2, q2) <=> 
   Holds(rext(f, r1, r2), rsi(r1, a), App(i2, q2))’
- >-- cheat >>
+ >-- (strip_tac >> pop_assum (assume_tac o GSYM) >> arw[]) >>
  rw[rext_def] >> strip_tac >> dimp_tac >> strip_tac (* 2 *)
- >-- (qexistsl_tac [‘a’,‘App(f,a)’] >> arw[]) >>
+ >-- (qexistsl_tac [‘a’,‘App(f,a)’] >> arw[]) >> 
  qsuff_tac ‘?b. App(i2, q2) = rsi(r2, b) & 
  Holds(r2,b,App(f, a))’ >-- 
  (strip_tac >> 
  qpick_x_assum ‘App(i2, q2) = rsi(r2, b')’
  (assume_tac o GSYM) >> arw[] >>
- qby_tac ‘Holds(r2,b,b')’ >-- cheat (*by assum*) >>
- cheat) >>
+ drule rsi_eq_ER >> arw[] >>
+ rev_drule rsi_eq_ER >> fs[] >> last_x_assum drule >>
+ rfs[]) >>
  qexists_tac ‘b’ >> arw[] >> pop_assum (assume_tac o GSYM) >>
- arw[] >> first_x_assum irule >> cheat
- (*final cheat by assum rsi(r1, a) = rsi(r1, a') *))
+ arw[] >> first_x_assum irule >> 
+ rev_drule rsi_eq_ER >> fs[ER_def,Sym_def] >> 
+ first_x_assum irule >> arw[])
 (form_goal
 “!A B f:A->B r1:A~>A r2:B~>B
  Q1 Q2 i1:Q1->Pow(A) i2:Q2->Pow(B). 
@@ -303,51 +386,67 @@ e0
  ?qf: Q1-> Q2.
  !q1:mem(Q1). Holds(rext(f,r1,r2),App(i1,q1),App(i2 o qf,q1)) ”));
 
-val main = prove_store("main",
-e0
-cheat
-(form_goal
-“!A B f:A->B r1:A~>A r2:B~>B
- Q1 Q2 i1:Q1->Pow(A) i2:Q2->Pow(B). 
- ER(r1) & ER(r2) & resp(f,r1,r2) &
- (!sa. (?q1. sa = App(i1,q1)) <=> (?a. sa = rsi(r1,a))) & 
- (!sb. (?q2. sb = App(i2,q2)) <=> (?b. sb = rsi(r2,b))) ==>
- ?qf: Q1-> Q2.
- !q1:mem(Q1). Holds(rext(f,r1,r2),App(i1,q1),App(i2 o qf,q1)) ”));
 
 
+(* Pow(A) * Pow(A) -> Pow(A * A) not have in general. *)
+
+val ipow2_def = P2fun' |> qspecl [‘Q1 * Q2’,‘Pow(A * B)’] 
+                     |> fVar_sInst_th “P(aqbq:mem(Q1 * Q2),s:mem(Pow(A * B)))”
+                        “!a1 a2.IN(Pair(a1,a2),s:mem(Pow(A * B))) <=> 
+                         IN(a1,App(i1:Q1-> Pow(A),Fst(aqbq))) & 
+                         IN(a2,App(i2:Q2-> Pow(B),Snd(aqbq)))”
+                     |> C mp 
+                     (IN_def_P |> qspecl [‘A * B’] 
+                               |> fVar_sInst_th “P(ab:mem(A * B))”
+                               “IN(Fst(ab),App(i1:Q1->Pow(A),Fst(aqbq))) & 
+                               IN(Snd(ab),App(i2:Q2->Pow(B),Snd(aqbq)))”
+                               |> conv_rule (depth_fconv no_conv 
+                                                         forall_cross_fconv)
+                               |> rewr_rule[Pair_def']
+                               |> qgen ‘aqbq’)
+                     |> qSKOLEM "ipow2" [‘i1’,‘i2’]
+                     |> conv_rule (depth_fconv no_conv forall_cross_fconv)
+                     |> rewr_rule[Pair_def']
+                     |> qspecl [‘aq:mem(Q1)’,‘bq:mem(Q2)’,
+                                ‘a:mem(A)’,‘b:mem(B)’] 
+                     |> gen_all |> store_as "ipow2_def";
 
 (*
-
-Pow(A) * Pow(A) -> Pow(A * A) not have in general.
-
- *)
-
-
 val ipow2_ex = prove_store("ipow2_ex",
 e0
-cheat
+(rpt strip_tac >> irule l >> rpt strip_tac >>
+ uex_tac)
 (form_goal “!i1:Q1-> Pow(A) i2:Q2 -> Pow(B). 
  ?i: Q1 * Q2 -> Pow(A * B).
  !aq bq.
   !a1 a2.IN(Pair(a1,a2),App(i,Pair(aq,bq))) <=> 
          IN(a1,App(i1,aq)) & IN(a2,App(i2,bq))”));
-
+end
 
 val ipow2_def = ipow2_ex |> spec_all 
                          |> qSKOLEM "ipow2" [‘i1’,‘i2’]
                          |> gen_all
-
-
-
+*)
+ 
+local 
+val l = P2fun' |> qspecl [‘(N * N) * N * N’,‘N * N’]
+       |> fVar_sInst_th “P(xyuv:mem((N * N) * N * N),ab:mem(N * N))”
+                        “ab  = Pair(Add(Fst(Fst(xyuv)),Fst(Snd(xyuv))),
+                                   Add(Snd(Fst(xyuv)),Snd(Snd(xyuv))))”
+       |> conv_rule (depth_fconv no_conv forall_cross_fconv) 
+       |> conv_rule (basic_fconv no_conv forall_cross_fconv) 
+       |> rewr_rule[Pair_def']
+in    
 val addf0_def = proved_th $
 e0
-cheat
+(irule l >> rpt strip_tac >> uex_tac >>
+ qexists_tac ‘Pair(Add(a', a), Add(b, b''))’ >> rw[])
 (form_goal “?f:(N * N) * N * N -> N * N. 
  !x y u v. App(f,Pair(Pair(x,y),Pair(u,v))) = 
  Pair(Add(x,u),Add(y,v))”)
 |> qSKOLEM "addf0" []
 |> store_as "addf0_def";
+end
 
 
 val negf0_def = fun_tm_compr (dest_var $ rastt "mn:mem(N * N)")
@@ -360,10 +459,230 @@ val negf0_def1 =
               |> rewr_rule[Pair_def']
               |> gen_all |> store_as "negf0_def1";
 
+val prrel_ER_ER = prove_store("prrel_ER_ER",
+e0
+(rpt strip_tac >> fs[ER_def,Sym_def,Trans_def,Refl_def] >> 
+ depth_fconv_tac no_conv forall_cross_fconv >> once_rw[prrel_def] >>
+ rpt strip_tac >> arw[] (* 4 *)
+ >-- (last_x_assum drule >> arw[]) 
+ >-- (first_x_assum drule >> arw[])
+ >-- (first_x_assum irule >> qexists_tac ‘a'’ >> arw[]) >>
+ first_x_assum irule >> qexists_tac ‘b'’ >> arw[])
+(form_goal “∀A r1:A~>A B r2:B~>B. ER(r1) & ER(r2) ⇒ ER(prrel(r1,r2))”));
+
+
+val forall_cross_tac =  depth_fconv_tac no_conv forall_cross_fconv;
+
+
+val Pow_conj_eq0 = prove_store("Pow_conj_eq0",
+e0
+(rpt strip_tac >>
+rw[GSYM IN_EXT_iff] >> strip_tac >> cases_on “IN(x,s1:mem(Pow(A)))”
+>-- (arw[] >> 
+    qsuff_tac ‘IN(x,s3) & IN(b0,s4)’ 
+    >-- (strip_tac >> arw[]) >>
+    first_x_assum (irule o iffLR) >> arw[]) >>
+arw[] >> ccontra_tac >>
+qby_tac ‘IN(b0,s4)’ 
+>-- (qsuff_tac ‘IN(a0,s3) & IN(b0,s4)’ 
+     >-- (strip_tac >> arw[]) >>
+     first_x_assum (irule o iffLR) >> arw[]) >>
+first_x_assum (qspecl_then [‘x’,‘b0’] assume_tac) >>
+rfs[])
+(form_goal “∀A B s1:mem(Pow(A)) s2:mem(Pow(B)) s3 s4 a0 b0. IN(a0,s1) & IN(b0,s2) ⇒  (∀a b. IN(a,s1) & IN(b,s2) ⇔ IN(a,s3) & IN(b,s4)) ⇒
+ s1 = s3”) );
+
+val Pow_conj_eq = prove_store("Pow_conj_eq",
+e0
+(rpt strip_tac 
+ >-- (irule Pow_conj_eq0 (* irule weird behaviour *)>>
+     rpt strip_tac >-- (qexists_tac ‘a0’ >> arw[]) >>
+     qexistsl_tac [‘B’,‘b0’,‘s2’,‘s4’] >> arw[]) >>
+ irule Pow_conj_eq0 >> rpt strip_tac (* 2 *)
+ >-- (qexists_tac ‘b0’ >> arw[]) >>
+ qexistsl_tac [‘A’,‘a0’,‘s1’,‘s3’] >> arw[] >> 
+ rpt strip_tac >> dimp_tac >> disch_tac (* 2 *)
+ >-- (qsuff_tac ‘IN(b, s3) & IN(a, s4)’ >-- (strip_tac >> arw[]) >>
+      first_x_assum (irule o iffLR) >> arw[]) >>
+ qsuff_tac ‘IN(b, s1) & IN(a,s2)’ >-- (strip_tac >> arw[]) >>
+ first_x_assum (irule o iffRL) >> arw[])
+(form_goal “∀A B s1:mem(Pow(A)) s2:mem(Pow(B)) s3 s4 a0 b0. IN(a0,s1) & IN(b0,s2) ⇒  (∀a b. IN(a,s1) & IN(b,s2) ⇔ IN(a,s3) & IN(b,s4)) ⇒
+ s1 = s3 & s2 = s4”));
+
+
+(*
+e0
+
+(rpt strip_tac >> rw[GSYM IN_EXT_iff] (* 2 *) >> strip_tac >--
+ (first_assum (qsspecl_then [‘x’,‘b0’] assume_tac) >> fs[] >>
+ cases_on “IN(x:mem(A), s1)” >-- fs[] >>
+ arw[] >> ccontra_tac >> rfs[] >> 
+ cases_on “IN(a0:mem(A),s3)” (* 2 *) >-- cheat
+>-- (first_assum (qsspecl_then [‘a0’,‘b0’] assume_tac) >>
+     qby_tac ‘IN(a0, s3) & IN(b0,s4)’
+     >-- (first_x_assum (irule o iffLR) >> strip_tac >> 
+                        first_x_assum accept_tac) >>
+     BUGBUGBUGBUGBUG!!!!!!!!!!!!!!!!!!!! CANNOT DO THE fs[], can finish the qby. if do the fs, complains
+ERR
+     ("disjE.first disjunct not in the formula list: ", [], [],
+      [Pred ("IN", true, [a0, s3])]) raised
+
+
+     fs[] >> first_x_assum (qspecl_then [‘x’,‘b0’] assume_tac) >> 
+     pop_assum mp_tac >> arw[]rfs[]) >>
+cheat)
+
+(form_goal “∀A B s1:mem(Pow(A)) s2:mem(Pow(B)) s3 s4 a0 b0. IN(a0,s1) & IN(b0,s2) ⇒  (∀a b. IN(a,s1) & IN(b,s2) ⇔ IN(a,s3) & IN(b,s4)) ⇒
+ s1 = s3 & s2 = s4”)
+
+*)
+
+val ipow2_Inj_Inj = prove_store("ipow2_Inj_Inj",
+e0
+(rpt strip_tac >> fs[Inj_def] >> 
+ depth_fconv_tac no_conv forall_cross_fconv >>
+ rw[GSYM IN_EXT_iff] >>
+ forall_cross_tac >> rpt strip_tac >> fs[ipow2_def] >>
+ rw[Pair_eq_eq] >> 
+ qsuff_tac ‘App(i1,a) = App(i1,a') & App(i2,b) = App(i2,b')’ 
+ >-- (rpt strip_tac >> first_x_assum irule >> arw[]) >>
+ irule Pow_conj_eq >> arw[])
+(form_goal “∀Q1 A i1:Q1 -> Pow(A) Q2 B i2:Q2->Pow(B). 
+ (∀q1. ∃a. IN(a,App(i1,q1))) &
+ (∀q2. ∃b. IN(b,App(i2,q2))) & 
+ Inj(i1) & Inj(i2) ⇒ Inj(ipow2(i1,i2))”));
+
+
+
+val Quo_def = qdefine_psym ("Quo",[‘r:A~>A’,‘i:Q->Pow(A)’])
+‘!s. (?!q. s = App(i:Q->Pow(A),q)) <=> (?a. s = rsi(r:A~>A,a))’
+|> gen_all |> store_as "Quo_def";
+
+val Inj_Quo = prove_store("Inj_Quo",
+e0
+(dimp_tac >> strip_tac >> arw[] (* 2 *)
+>-- (rw[Quo_def] >> strip_tac >> dimp_tac >> strip_tac (* 2 *)
+    >-- (pop_assum (assume_tac o uex2ex_rule) >>
+        first_x_assum (drule o iffLR) >> arw[]) >>
+    uex_tac >> 
+    qby_tac ‘∃a. s = rsi(r,a)’ >-- (qexists_tac ‘a’ >> arw[]) >>
+    first_x_assum (drule o iffRL) >> pop_assum strip_assume_tac >>
+    qexists_tac ‘q’ >> fs[Inj_def] >> rpt strip_tac >>
+    first_x_assum irule >> arw[]) >>
+fs[Quo_def] >> strip_tac >> dimp_tac >> strip_tac (* 2 *)
+>-- (qby_tac ‘∃!q.s = App(i,q)’
+    >-- (uex_tac >> qexists_tac ‘q’ >> arw[] >> rpt strip_tac >>
+        fs[Inj_def] >> first_x_assum irule >> arw[]) >>
+    first_x_assum (drule o iffLR) >> arw[]) >>
+qsuff_tac ‘∃!q. s = App(i,q)’ 
+>-- (strip_tac >> pop_assum (assume_tac o uex2ex_rule) >> arw[]) >>
+first_x_assum (irule o iffRL) >> qexists_tac ‘a’ >> arw[])
+(form_goal
+“(Inj(i) & !s. (?q. s = App(i:Q->Pow(A),q)) <=> (?a. s = rsi(r:A~>A,a)))
+ ⇔ Inj(i) & Quo(r,i)”));
+
+val ER_rsi_nonempty = prove_store("ER_rsi_nonempty",
+e0
+(rpt strip_tac >> rw[IN_rsi] >> fs[ER_def,Refl_def])
+(form_goal “∀A r:A~>A a:mem(A).ER(r) ⇒ IN(a,rsi(r,a)) ”));
+
+val Quo_cong = prove_store("Quo_cong",
+e0
+(rpt strip_tac >> fs[Quo_def] >> 
+ depth_fconv_tac no_conv exists_cross_fconv >>
+ rw[GSYM IN_EXT_iff] >>
+ depth_fconv_tac no_conv forall_cross_fconv >> 
+ rw[IN_rsi,prrel_def,ipow2_def] >> strip_tac >> dimp_tac >> strip_tac (* 2 *)
+ >-- (qby_tac
+     ‘∀a. ∃!q.rsi(r1,a) = App(i1,q)’
+     >-- (strip_tac >>
+         qby_tac ‘∃a1. rsi(r1,a) = rsi(r1,a1)’ 
+         >-- (qexists_tac ‘a’ >> rw[]) >>
+         first_x_assum (drule o iffRL) >> arw[]) >>
+     qby_tac
+     ‘∀b. ∃!q.rsi(r2,b) = App(i2,q)’
+     >-- (strip_tac >>
+         qby_tac ‘∃b1. rsi(r2,b) = rsi(r2,b1)’ 
+         >-- (qexists_tac ‘b’ >> rw[]) >>
+         first_x_assum (drule o iffRL) >> arw[])  >>
+     first_x_assum (assume_tac o uex_expand) >>
+     pop_assum (x_choose_then "q12" strip_assume_tac) >>
+     arw[] >> 
+     qsspecl_then [‘q12’] (x_choosel_then ["q1","q2"] assume_tac) 
+     Pair_has_comp >> fs[] >>
+     rw[ipow2_def] >> rw[GSYM IN_rsi] >>
+     qsuff_tac ‘∃a1 b1. App(i1, q1) = rsi(r1, a1) & App(i2,q2) = rsi(r2, b1)’ 
+     >-- (strip_tac >> qexistsl_tac [‘a1’,‘b1’] >> arw[]) >>
+     qby_tac ‘∃!q. App(i1,q1) = App(i1,q)’ 
+     >-- (uex_tac >> qexists_tac ‘q1’ >> rw[] >> fs[Inj_def] >>
+         rpt strip_tac >> first_x_assum irule >> arw[]) >>
+     first_x_assum (drule o iffLR) >> pop_assum strip_assume_tac >>
+     qby_tac ‘∃!q. App(i2,q2) = App(i2,q)’ 
+     >-- (uex_tac >> qexists_tac ‘q2’ >> rw[] >> fs[Inj_def] >>
+         rpt strip_tac >> first_x_assum irule >> arw[]) >>
+     first_x_assum (drule o iffLR) >> pop_assum strip_assume_tac >>
+     qexistsl_tac [‘a’,‘a'’] >> arw[]) >>
+qsuff_tac ‘∃!q:mem(Q1 * Q2).
+ (∀a1 b1. Holds(r1, a', a1) & Holds(r2, b, b1) ⇔ 
+  IN(Pair(a1, b1), App(ipow2(i1, i2), q)))’
+>-- (strip_tac >> pop_assum (strip_assume_tac o  uex_expand) >>
+    uex_tac >> qexists_tac ‘q’ >> rpt strip_tac >> arw[] >>
+    first_x_assum irule >> fs[]) 
+(*this qsuff not automatic, MAY HAVE BUG IN FORALL_FCONV!!!!!!*) >>
+qby_tac ‘∃a. rsi(r1,a') = rsi(r1,a)’ 
+>-- (qexists_tac ‘a'’ >> rw[]) >>
+first_x_assum (drule o iffRL) >> 
+pop_assum (assume_tac o uex_expand) >>
+pop_assum (x_choose_then "q1" strip_assume_tac) >>
+qby_tac ‘∃b1. rsi(r2,b) = rsi(r2,b1)’ 
+>-- (qexists_tac ‘b’ >> rw[]) >>
+first_x_assum (drule o iffRL) >> 
+pop_assum (assume_tac o uex_expand) >>
+pop_assum (x_choose_then "q2" strip_assume_tac) >>
+uex_tac >> qexists_tac ‘Pair(q1,q2)’ >> 
+depth_fconv_tac no_conv forall_cross_fconv >>
+rw[ipow2_def,GSYM IN_rsi,Pair_eq_eq] >>
+qsuff_tac ‘rsi(r1, a') = App(i1, q1) & rsi(r2, b) = App(i2, q2)’
+>-- (strip_tac >> arw[] >> rpt gen_tac >> disch_tac >>
+    qsuff_tac ‘App(i1, q1) = App(i1, a) & 
+               App(i2, q2) = App(i2, b')’ 
+    >-- (rpt strip_tac >> fs[Inj_def] >> first_x_assum irule >> arw[]) >>
+    irule Pow_conj_eq >>
+    arw[] >> strip_tac (* 2 *)
+    >-- (qexists_tac ‘b’ >> 
+        qpick_x_assum ‘rsi(r2, b) = App(i2, q2)’ (assume_tac o GSYM) >>
+        arw[] >> irule ER_rsi_nonempty >> arw[]) >>
+    qexists_tac ‘a'’ >> 
+    qpick_x_assum ‘rsi(r1, a') = App(i1, q1)’ (assume_tac o GSYM) >>
+    arw[] >> irule ER_rsi_nonempty >> arw[]) >>
+arw[])
+(form_goal “∀A r1:A~>A Q1 i1:Q1-> Pow(A) B r2:B~>B Q2 i2:Q2 -> Pow(B). 
+ ER(r1) & ER(r2) & Inj(i1) & Inj(i2) &
+ Quo(r1,i1) & Quo(r2,i2) ⇒
+ Quo(prrel(r1,r2),ipow2(i1,i2))”));
+
+
+val Quo_fun = prove_store("Quo_fun",
+e0
+(rpt strip_tac >> 
+ irule main >> arw[] >> strip_tac (* 2 *)
+ >-- (qby_tac ‘Inj(i1) & Quo(r1,i1)’ 
+     >-- arw[] >>
+     drule (iffRL Inj_Quo) >> arw[]) >>
+ qby_tac ‘Inj(i2) & Quo(r2,i2)’ 
+ >-- arw[] >>
+ drule (iffRL Inj_Quo) >> arw[])
+(form_goal
+“!A B f:A->B r1:A~>A r2:B~>B
+ Q1 Q2 i1:Q1->Pow(A) i2:Q2->Pow(B). 
+ ER(r1) & ER(r2) & resp(f,r1,r2) & Inj(i1) & Inj(i2) &
+ Quo(r1,i1) & Quo(r2,i2) ==>
+ ?qf: Q1-> Q2.
+ !q1:mem(Q1). Holds(rext(f,r1,r2),App(i1,q1),App(i2 o qf,q1)) ”))
 
 
 val main_addz = 
-main |> qspecl [‘(N * N) * (N * N)’,‘N * N’,
+Quo_fun |> qspecl [‘(N * N) * (N * N)’,‘N * N’,
                 ‘addf0’,
                 ‘prrel(ZR,ZR)’,‘ZR’,
                 ‘Z * Z’,‘Z’,
